Protocols/RB/Liveness.v
@@ -29,8 +29,29 @@ Set Implicit Arguments. (* anyway *)
 (* at the beginning *)
 Definition some_receives src r v w : Prop := exists n, is_byz n = false /\ In v ((w @ n).(output) (src, r)).
 
+(* Definition nonfaulty_bcast src r w : Prop := is_byz src = false /\ (w @ src).(sent) r. *)
+
 (* at the end *)
 Definition all_receives src r v w : Prop := forall n, is_byz n = false -> In v ((w @ n).(output) (src, r)).
+
+Definition pkts_needed size w nonbyz_senders pkts (m : Message) (P : World -> Address -> Prop) : Prop :=
+  List.NoDup nonbyz_senders /\
+  size <= length nonbyz_senders /\
+  incl pkts (sentMsgs w) /\
+  Forall good_packet pkts /\ (* since pkts is under-specified *)
+  (forall n1,
+    In n1 nonbyz_senders -> 
+    is_byz n1 = false /\
+    P w n1 /\
+    (forall n2, is_byz n2 = false ->
+      exists used, In (mkP n1 n2 m used) pkts)).
+
+Definition mutual_receiving m w' :=
+  forall n1, is_byz n1 = false -> 
+    forall n2, is_byz n2 = false ->
+      In (mkP n1 n2 m true) (sentMsgs w').
+
+Module Global_Liveness.
 
 Section Proof_of_Global_Liveness.
 
@@ -39,18 +60,8 @@ Section Proof_of_Global_Liveness.
   Section Prelude.
 
   (* the structure of Round 1 and Round 2 are similar, so some conclusions might be reused *)
-
-  Definition pkts_needed size w nonbyz_senders pkts : Prop :=
-    List.NoDup nonbyz_senders /\
-    size <= length nonbyz_senders /\
-    incl pkts (sentMsgs w) /\
-    Forall good_packet pkts /\ (* since pkts is under-specified *)
-    (forall n1,
-      In n1 nonbyz_senders -> 
-      is_byz n1 = false /\
-      (w @ n1).(voted) (src, r) = Some v /\
-      (forall n2, is_byz n2 = false ->
-        exists used, In (mkP n1 n2 (ReadyMsg src r v) used) pkts)).
+  Definition pkts_needed size w nonbyz_senders pkts :=
+    pkts_needed size w nonbyz_senders pkts (ReadyMsg src r v) (fun w n => (w @ n).(voted) (src, r) = Some v).
 
   Lemma pkts_needed_by_voted_nodes w size (H_w_reachable : reachable w)
     nonbyz_senders (Hf_nonbyz : forall n, In n nonbyz_senders -> is_byz n = false)
@@ -110,14 +121,11 @@ Section Proof_of_Global_Liveness.
   Variable (nonbyz_senders : list Address) (pkts : list Packet).
   Hypotheses (Hround1 : pkts_needed_in_round_1 nonbyz_senders pkts).
 
+  (* FIXME: this might be rewritten as mutual_receiving *)
   Definition round_1_end w' :=
     forall n1, In n1 nonbyz_senders -> 
       forall n2, is_byz n2 = false ->
         In (mkP n1 n2 (ReadyMsg src r v) true) (sentMsgs w').
-
-  (* at the same time as round 1 ends *)
-  Definition round_2_start w' :=
-    forall n, is_byz n = false -> (w' @ n).(voted) (src, r) = Some v.
 
   Fact round_1_end_suffcond w' (Hincl : incl (map receive_pkt pkts) (sentMsgs w')) :
     round_1_end w'.
@@ -126,6 +134,10 @@ Section Proof_of_Global_Liveness.
     hnf. intros n1 Hin1 n2 Hnonbyz_n2. specialize (HH _ Hin1).
     destruct HH as (_ & _ & HH). specialize (HH _ Hnonbyz_n2). destruct HH as (? & HH). now apply (in_map receive_pkt), Hincl in HH.
   Qed.
+
+  (* at the same time as round 1 ends *)
+  Definition round_2_start w' :=
+    forall n, is_byz n = false -> (w' @ n).(voted) (src, r) = Some v.
 
   Lemma round_2_start_suffcond w0 l0 (Htrace0 : system_trace w l0) (Ew0 : w0 = final_world w l0) 
     (Hw0 : round_1_end w0) : round_2_start w0.
@@ -178,9 +190,7 @@ Section Proof_of_Global_Liveness.
   Hypotheses (Hround2 : pkts_needed_in_round_2 nonbyz_senders pkts).
 
   Definition round_2_end w' :=
-    forall n1, is_byz n1 = false -> 
-      forall n2, is_byz n2 = false ->
-        In (mkP n1 n2 (ReadyMsg src r v) true) (sentMsgs w').
+    Eval unfold mutual_receiving in mutual_receiving (ReadyMsg src r v) w'.
 
   Fact round_2_end_suffcond w' (Hincl : incl (map receive_pkt pkts) (sentMsgs w')) :
     round_2_end w'.
@@ -211,8 +221,152 @@ Section Proof_of_Global_Liveness.
 
 End Proof_of_Global_Liveness.
 
+End Global_Liveness.
+
+Module Validity1.
+
 Section Proof_of_Validity1.
 
+  Variables (src : Address) (r : Round).
+  Hypothesis (Hnonbyz_src : is_byz src = false).
+
+  Section Round1.
+
+  Variable (w : World).
+  Hypotheses (H_w_reachable : reachable w) (Hstart : (w @ src).(sent) r).
+
+  Definition pkts_needed_in_round_1 pkts : Prop :=
+    incl pkts (sentMsgs w) /\
+    Forall good_packet pkts /\ (* since pkts is under-specified *)
+    (forall n, is_byz n = false ->
+      exists used, In (mkP src n (InitialMsg r (value_bft src r)) used) pkts).
+
+  Lemma round_1_pkts : exists pkts, pkts_needed_in_round_1 pkts.
+  Proof.
+    unfold pkts_needed_in_round_1. saturate.
+    exists (List.filter (fun p =>
+      (Message_eqdec p.(msg) (InitialMsg r (value_bft src r))) &&
+      (Address_eqdec (P.src p) src) && (negb (is_byz p.(dst)))) (sentMsgs w)).
+    split_and?; auto using incl_filter.
+    - apply Forall_forall. intros [ s d m b ] (Hin & Hcheck)%filter_In. simpl in Hcheck.
+      unfold is_left in Hcheck. rewrite ! andb_true_iff, ! negb_true_iff in Hcheck. hnf. destruct_eqdec in_ Hcheck as_ ?; try eqsolve. now simplify_eq.
+    - intros n Hnonbyz_n.
+      pick initialmsg_sent_fwd as_ H1 by_ (pose proof (Hfwd _ Hnonbyz_src) as []). specialize (H1 _ Hstart n). rewrite Hcoh in H1.
+      destruct H1 as (b & H1). exists b. unfold is_left. rewrite filter_In, ! andb_true_iff, negb_true_iff. simpl. now rewrite ! eqdec_refl.
+  Qed.
+
+  Variable (pkts : list Packet).
+  Hypotheses (Hround1 : pkts_needed_in_round_1 pkts).
+
+  Definition round_1_end w' :=
+    forall n, is_byz n = false -> In (mkP src n (InitialMsg r (value_bft src r)) true) (sentMsgs w').
+
+  Fact round_1_end_suffcond w' (Hincl : incl (map receive_pkt pkts) (sentMsgs w')) :
+    round_1_end w'.
+  Proof.
+    destruct Hround1 as (_ & _ & H2). 
+    hnf. intros n Hnonbyz_n. specialize (H2 _ Hnonbyz_n).
+    destruct H2 as (? & H2). now apply (in_map receive_pkt), Hincl in H2.
+  Qed.
+
+  (* at the same time as round 1 ends *)
+  Definition round_2_start w' :=
+    forall n, is_byz n = false -> (w' @ n).(echoed) (src, r) = Some (value_bft src r).
+
+  Lemma round_2_start_suffcond w0 l0 (Htrace0 : system_trace w l0) (Ew0 : w0 = final_world w l0) 
+    (Hw0 : round_1_end w0) : round_2_start w0.
+  Proof.
+    pose proof (reachable_by_trace Htrace0 H_w_reachable) as H_w0_reachable. rewrite <- Ew0 in H_w0_reachable.
+    clear H_w_reachable. saturate.
+
+    hnf in Hw0 |- *. intros n Hnonbyz_n. specialize (Hw0 _ Hnonbyz_n).
+    pick initialmsg_recv_bwd as_ Hp by_ (pose proof (Hbwdr _ Hw0) as []). saturate_assumptions.
+    destruct (echoed _ _) as [ v' | ] eqn:Ev' in |- *; [ | isSome_rewrite; discriminate ].
+    (* TODO the following two steps are repeating in the integrity proof *)
+    pick initialmsg_recv_fwd as_ H4 by_ (pose proof (Hfwd _ Hnonbyz_n) as []). specialize (H4 _ _ _ Ev'). rewrite Hcoh in H4.
+    pick initialmsg_sent_bwd as_ H5 by_ (pose proof (Hbwds _ H4) as []). saturate_assumptions. now f_equal.
+  Qed.
+
+  End Round1.
+
+  Section Round2.
+
+  Variable (w : World).
+  Hypotheses (H_w_reachable : reachable w) (Hstart : round_2_start w).
+
+  Definition pkts_needed_in_round_2 nonbyz_senders pkts : Prop :=
+    Eval unfold pkts_needed in pkts_needed (N - t0) w nonbyz_senders pkts (EchoMsg src r (value_bft src r))
+      (fun w n => (w @ n).(echoed) (src, r) = Some (value_bft src r)).
+
+  Let nonbyz_senders := (List.filter (fun n => negb (is_byz n)) valid_nodes).
+
+  (* in the second round, there are (N-t0) non-faulty nodes broadcasting Echo messages *)
+  Lemma round_2_pkts :
+    exists pkts, pkts_needed_in_round_2 nonbyz_senders pkts.
+  Proof.
+    unfold pkts_needed_in_round_2, nonbyz_senders. saturate.
+    exists (List.filter (fun p => 
+      match p.(msg) with
+      | EchoMsg _ _ _ => (negb (is_byz (P.src p))) && (negb (is_byz p.(dst)))
+      | _ => false
+      end) (sentMsgs w)).
+    hnf. split_and?; auto using incl_filter, NoDup_filter, valid_nodes_NoDup, nonbyz_lower_bound.
+    - apply Forall_forall. intros [ s d [] b ] (Hin & Hcheck)%filter_In; simpl in Hcheck; try discriminate.
+      now rewrite andb_true_iff, ! negb_true_iff in Hcheck.
+    - intros n1 (_ & Hnonbyz_n1)%filter_In. rewrite negb_true_iff in Hnonbyz_n1.
+      hnf in Hstart. specialize (@Hstart _ Hnonbyz_n1). (* TODO why @? *) split_and?; auto.
+      intros n2 Hnonbyz_n2.
+      pick echomsg_sent_fwd as_ Hsent1 by_ (pose proof (Hfwd _ Hnonbyz_n1) as []). specialize (Hsent1 _ _ _ Hstart n2). rewrite Hcoh in Hsent1.
+      destruct Hsent1. eexists. apply filter_In. 
+      simpl. split; [ eassumption | now rewrite andb_true_iff, ! negb_true_iff ].
+  Qed.
+
+  (* universally quantified *)
+  Variable (pkts : list Packet).
+  Hypotheses (Hround2 : pkts_needed_in_round_2 nonbyz_senders pkts).
+
+  Definition round_2_end w' :=
+    Eval unfold mutual_receiving in mutual_receiving (EchoMsg src r (value_bft src r)) w'.
+
+  (* FIXME: this is repeating *)
+  Fact round_2_end_suffcond w' (Hincl : incl (map receive_pkt pkts) (sentMsgs w')) :
+    round_2_end w'.
+  Proof.
+    hnf in Hround2. pick EchoMsg as_ HH by_ (destruct_and? Hround2).
+    hnf. intros n1 Hin1 n2 Hnonbyz_n2. 
+    specialize (HH n1 ltac:(unfold nonbyz_senders; rewrite filter_In, negb_true_iff; auto using Address_is_finite)).
+    destruct HH as (_ & _ & HH). specialize (HH _ Hnonbyz_n2). destruct HH as (? & HH). now apply (in_map receive_pkt), Hincl in HH.
+  Qed.
+
+  (* at the same time as round 2 ends *)
+  Definition round_3_start :=
+    Eval unfold Global_Liveness.round_2_start in Global_Liveness.round_2_start src r (value_bft src r).
+
+  Lemma round_3_start_suffcond w0 l0 (Htrace0 : system_trace w l0) (Ew0 : w0 = final_world w l0) 
+    (Hw0 : round_2_end w0) : round_3_start w0.
+  Proof.
+    pose proof (reachable_by_trace Htrace0 H_w_reachable) as H_w0_reachable. rewrite <- Ew0 in H_w0_reachable.
+    clear H_w_reachable. saturate.
+
+    hnf in Hw0 |- *. intros n Hnonbyz_n. 
+    hnf in Hround2. destruct Hround2 as (Hnodup & Hsize & _ & _ & HH).
+    destruct (voted _ _) as [ v' | ] eqn:Ev' in |- *.
+    - (* use vote_integrity *)
+      f_equal.
+      pose proof (vote_integrity_is_safety H_w0_reachable) as Htmp. now eapply (Htmp n src) in Ev'; try eassumption.
+    - (* prove contradiction using the message size *)
+      (* TODO repeating *)
+      pick voted_coh_none as_ Hp by_ (pose proof (Hst n) as []). apply Hp with (v:=value_bft src r) in Ev'.
+      assert (incl nonbyz_senders (msgcnt (w0 @ n) (EchoMsg src r (value_bft src r)))) as Hincl.
+      { hnf. subst nonbyz_senders. intros nn (_ & Hnonbyz_nn%negb_true_iff)%filter_In. specialize (Hw0 nn ltac:(assumption) n ltac:(assumption)).
+        pick msgcnt_recv_bwd as_ Hr by_ (pose proof (Hbwdr _ Hw0) as []). saturate_assumptions. now simpl in Hr. }
+      apply NoDup_incl_length in Hincl; try assumption. unfold th_echo4ready in Ev'. destruct Ev'. lia.
+  Qed.
+
+  End Round2.
+
 End Proof_of_Validity1.
+
+End Validity1.
 
 End RBLiveness.
